fix compilation

theories/L/TM/TimeInvarianceTermination.v
@@ -12,11 +12,13 @@ Require Import Undecidability.L.Util.L_facts.
 From Undecidability.L.Datatypes Require Import LNat.
 
 Import L_Notations.
-Import HOAS_Notations.
 
 Notation PAIR := (lam (lam (lam (0 2 1)))).
+Notation PAIR_ x y := (lam (0 x y)).
 
 Section TimeInvarianceNF.
+
+Import HOAS_Notations.
 
 Variable Σ : finType.
 
@@ -36,16 +38,16 @@ Existing Instance reg_state.
 Definition step_fun := (fun cfg : mconfig Σ (state M) n_tps =>
                           if haltConf cfg then inr (ctapes cfg) else inl (TM_facts.step cfg)).
 
-Notation STEPTIME := (haltTime M + n_tps* 130+ transTime M + 185).
+Notation STEPTIME := (haltTime M + n_tps* 130+ transTime M + 185). 
 
 Instance step_fun_comp : computableTime' step_fun (fun _ _ => (STEPTIME,tt)).
 Proof.
-  extract. solverec.
+  extract. solverec. 
 Qed.
 
 Lemma TimeInvarianceNF_forward i :
     loopSumM (M := M) (mk_mconfig q t) i = Some (mk_mconfig q' t') ->
-    evalLe (9 + i * (STEPTIME + 11) ) (s_sim ((PAIR (ext step_fun)) (enc q)) (enc t)) (enc t').
+    evalLe (7 + i * (STEPTIME + 11) ) (s_sim (PAIR_ (ext step_fun) (enc q)) (enc t)) (enc t').
 Proof.
   intros H.
   assert (Hi : loopSum i step_fun (mk_mconfig q t) = Some t').
@@ -71,10 +73,10 @@ Proof.
 Qed.
 
 Lemma TimeInvarianceNF_backward v :
-  eval (s_sim ((PAIR (ext step_fun)) (enc q)) (enc t)) v -> exists q' t' i, loopSumM (M := M) (mk_mconfig q t) i = Some (mk_mconfig q' t').
+  eval (s_sim (PAIR_ (ext step_fun) (enc q)) (enc t)) v -> exists q' t' i, loopSumM (M := M) (mk_mconfig q t) i = Some (mk_mconfig q' t').
 Proof.
   intros H.
-  assert ((s_sim ((PAIR (ext step_fun)) (enc q)) (enc t)) >* uiter (ext step_fun) (lam (O (enc q) (enc t)))).
+  assert ((s_sim (PAIR_ (ext step_fun) (enc q)) (enc t)) >* uiter (ext step_fun) (lam (O (enc q) (enc t)))).
   { clear H.
     unfold s_sim. now Lsimpl. }
   rewrite H0 in H. clear H0.
@@ -98,33 +100,68 @@ End TimeInvarianceNF.
 
 Definition sizeTM Σ n (M : TM Σ n) := (haltTime M + n* 130+ transTime M + 185 + 11).
 
-Theorem TimeInvarianceThesis_wrt_Termination_TM_to_L :
-  forall n Σ, exists encTM : TM Σ n -> term, exists encTps : tapes Σ n -> term,
-      exists sₛᵢₘ : term, exists C1 C2 : nat, forall M : TM Σ n, forall tps,
-              (forall tps' i q',
-                  loopM (mk_mconfig (start M) tps) i = Some (mk_mconfig q' tps') ->
-                  evalLe (C1 * (S i) * sizeTM M + C2) (sₛᵢₘ (encTM M) (encTps tps)) (encTps tps')) /\
-              (forall v, eval (sₛᵢₘ (encTM M) (encTps tps)) v -> exists q' tps' i, loopM (mk_mconfig (start M) tps) i = Some (mk_mconfig q' tps')).
+Definition encTM {n} {Σ : finType} : TM Σ n -> term.
 Proof.
-  intros n Σ.
   pose (reg_sig := @registered_finType Σ).
-  unshelve eexists.
-  { intros M.
-    pose (reg_state := @registered_finType (state M)).
-    unshelve refine (PAIR (extT (step_fun (M := M))) (enc (start M))). 3:eapply step_fun_comp.
-  }
-  unshelve eexists.
-  { intros tps. exact (enc tps). }
-  exists s_sim.
-  eexists 10, 10.
+  intros M.
+  pose (reg_state := @registered_finType (state M)).
+  unshelve refine (PAIR_ (extT (step_fun (M := M))) (enc (start M))). 3:eapply step_fun_comp.
+Defined.
+
+Definition encTps  {n} {Σ : finType} : tapes Σ n -> term.
+Proof.
+  pose (reg_sig := @registered_finType Σ).
+  intros tps. exact (enc tps).  
+Defined.
+
+Theorem TimeInvarianceThesis_wrt_Termination_TM_to_L : let C := 10 in
+  forall n (Σ : finType), forall M : TM Σ n, forall tps,
+          (forall tps' i q',
+              loopM (mk_mconfig (start M) tps) i = Some (mk_mconfig q' tps') ->
+              evalLe (C * (S i) * sizeTM M + C) (s_sim (encTM M) (encTps tps)) (encTps tps')) /\
+          (forall v, eval (s_sim (encTM M) (encTps tps)) v -> exists q' tps' i, loopM (mk_mconfig (start M) tps) i = Some (mk_mconfig q' tps')).
+Proof.
+  intros C n Σ. subst C.
+  pose (reg_sig := @registered_finType Σ).
   intros M tps. split.
   - intros tps' i q' H.
     rewrite loopSumM_loopM_iff in H.
     eapply TimeInvarianceNF_forward in H.
-    eapply evalLe_trans_rev with (k := 9) in H as (H1 & H & _).
+    eapply evalLe_trans_rev with (k := 7) in H as (H1 & H & _).
     2:{ unfold s_sim. Lsimpl. } cbn -[mult].
-    unfold s_sim. 
+    unfold s_sim. unfold encTM, encTps.
     eapply evalIn_mono. Lsimpl. eapply (evalIn_refl 0). Lproc.
     fold (sizeTM M). ring_simplify. lia.
   - intros v (q' & t' & [] & H) % TimeInvarianceNF_backward. inv H. setoid_rewrite loopSumM_loopM_iff. eauto.
 Qed.
+
+(* Theorem TimeInvarianceThesis_wrt_Termination_TM_to_L : *)
+(*   forall n Σ, exists encTM : TM Σ n -> term, exists encTps : tapes Σ n -> term, *)
+(*       exists sₛᵢₘ : term, exists C1 C2 : nat, forall M : TM Σ n, forall tps, *)
+(*               (forall tps' i q', *)
+(*                   loopM (mk_mconfig (start M) tps) i = Some (mk_mconfig q' tps') -> *)
+(*                   evalLe (C1 * (S i) * sizeTM M + C2) (sₛᵢₘ (encTM M) (encTps tps)) (encTps tps')) /\ *)
+(*               (forall v, eval (sₛᵢₘ (encTM M) (encTps tps)) v -> exists q' tps' i, loopM (mk_mconfig (start M) tps) i = Some (mk_mconfig q' tps')). *)
+(* Proof. *)
+(*   intros n Σ. *)
+(*   pose (reg_sig := @registered_finType Σ). *)
+(*   unshelve eexists. *)
+(*   { intros M. *)
+(*     pose (reg_state := @registered_finType (state M)). *)
+(*     unshelve refine (PAIR (extT (step_fun (M := M))) (enc (start M))). 3:eapply step_fun_comp. *)
+(*   } *)
+(*   unshelve eexists. *)
+(*   { intros tps. exact (enc tps). } *)
+(*   exists s_sim. *)
+(*   eexists 10, 10. *)
+(*   intros M tps. split. *)
+(*   - intros tps' i q' H. *)
+(*     rewrite loopSumM_loopM_iff in H. *)
+(*     eapply TimeInvarianceNF_forward in H. *)
+(*     eapply evalLe_trans_rev with (k := 9) in H as (H1 & H & _). *)
+(*     2:{ unfold s_sim. Lsimpl. } cbn -[mult]. *)
+(*     unfold s_sim.  *)
+(*     eapply evalIn_mono. Lsimpl. eapply (evalIn_refl 0). Lproc. *)
+(*     fold (sizeTM M). ring_simplify. lia. *)
+(*   - intros v (q' & t' & [] & H) % TimeInvarianceNF_backward. inv H. setoid_rewrite loopSumM_loopM_iff. eauto. *)
+(* Qed. *)
